\section{}





\subsection{}

Suppose that~$x_k \wto x$.
We then know from the lecture (Proposition~8.3, part~(iv)) that the sequence~$(x_k)_k$ is bounded.
The convergence~$\bil{x_k, x'} \to \bil{x, x'}$ holds for every~$x' \in X'$, whence for every~$x' \in D$.

Suppose now that the sequence~$(x_k)_k \subseteq X$ is bounded, say~$\norm{x_k} \leq C$ for every~$k$ for some~$C \geq 0$, and that there exists a dense subset~$D \subseteq X'$ with~$\bil{x_k, x'} \to \bil{x, x'}$ for every~$x' \in D$.

Let~$x' \in X'$.
There exists some~$\tilde{x}' \in D$ with
\[
  \norm{x} \norm{x' - \tilde{x}'} \leq \frac{\varepsilon}{2}
  \quad\text{and}\quad
  C \norm{\tilde{x'} - x'} \leq \frac{\varepsilon}{2}
\]
because~$D$ is dense in~$X'$.
It then holds that
\begin{align*}
  \abs{ \bil{x_k, x'} - \bil{x, x'} }
  &\leq
    \abs{ \bil{x_k, x'} - \bil{x_k, \tilde{x}'} }
  + \abs{ \bil{x_k, \tilde{x}'} - \bil{x, \tilde{x}'} }
  + \abs{ \bil{x, \tilde{x}'} - \bil{x, x'} } \\
  &=
      \abs{ \bil{x_k, x' - \tilde{x}' } }
    + \abs{ \bil{x_k, \tilde{x}'} - \bil{x, \tilde{x}' } }
    + \abs{ \bil{x, \tilde{x}' - x' } } \\
  &\leq
      \norm{x_k} \norm{x' - \tilde{x}'}
    + \abs{ \bil{x_k, \tilde{x}'} - \bil{x, \tilde{x}' } }
    + \norm{x} \norm{\tilde{x'} - x'} \\
  &\leq
      \frac{\varepsilon}{2}
    + \abs{ \bil{x_k, \tilde{x}'} - \bil{x, \tilde{x}' } }
    + \frac{\varepsilon}{2} \\
  &=  \abs{ \bil{x_k, \tilde{x}'} - \bil{x, \tilde{x}' } }
    + \varepsilon \,.
\end{align*}
When taking the limit~$k \to \infty$ we have by assumption that~$\abs{ \bil{x_k, \tilde{x}'} - \bil{x, \tilde{x}' } } \to 0$.
We hence find that
\[
        \limsup_{k \to \infty} \abs{ \bil{x_k, x'} - \bil{x, x'} }
  \leq  \varepsilon \,.
\]
This holds for every~$\varepsilon > 0$, whence~$\bil{x_k, x'} \to \bil{x,x'}$.
This shows that~$x_k \wto x$.





\subsection{}

Suppose that~$x_k \to x$.
Then
\begin{align*}
  \sup_{\norm{x'} = 1}
  \abs*{ \bil{x_k, x'} - \bil{x, x'} }
  &=
  \sup_{\norm{x'} = 1}
  \abs*{ \bil{x_k - x, x'} }
  \\
  &\leq
  \sup_{\norm{x'} = 1}
  \norm{x_k - x} \norm{x'}
  =
  \norm{x_k - x}
  \to
  0 \,.
\end{align*}

Suppose on the other hand that~$\sup_{\norm{x'} = 1} \abs{ \bil{x_k, x'} - \bil{x, x'} } \to 0$.
We know from the lecture (Corollary~6.6) that there exists for every~$k$ some~$x'_0 \in X'$ with~$\norm{x'_0} = 1$ such that
\[
    \bil{x_k - x, x'_0}
  = \norm{x_k - x} \,.
\]
Then
\[
        \norm{x_k - x}
   =    \abs{ \bil{x_k - x, x'_0} }
   =    \abs{ \bil{x_k, x'_0} - \bil{x, x'_0} }
   \leq \sup_{\norm{x'}  = 1} \abs{ \bil{x_k, x'} - \bil{x, x'} }
   \to  0 \,,
\]
which shows that~$x_k \to x$.




