\section{}

We consider only the case that~$\Omega$ is nonempty.





\subsection{}

It follows from~$\alpha < \beta$ and the boundedness of~$\Omega$ that
\[
            C
  \defined  \sup_{\substack{x, y \in \Omega \\ x \neq y}}
            \frac{1}{\norm{x - y}^{\alpha - \beta}}
  =         \sup_{\substack{x, y \in \Omega \\ x \neq y}}
            \norm{x - y}^{\beta - \alpha}
  <         \infty
\]
with~$C > 0$.
It therefore holds for every function~$f \colon \Omega \to \Real^m$ that
\begin{align*}
        [f]_{\alpha}
  &=    \sup_{\substack{x, y \in \Omega \\ x \neq y}}
        \frac{\norm{f(x) - f(y)}}{\norm{x - y}^\alpha}
   =    \sup_{\substack{x, y \in \Omega \\ x \neq y}}
        \frac{1}{\norm{x - y}^{\alpha - \beta}}
        \frac{\norm{f(x) - f(y)}}{\norm{x - y}^\beta} \\
  &\leq \sup_{\substack{x, y \in \Omega \\ x \neq y}}
        C
        \frac{\norm{f(x) - f(y)}}{\norm{x - y}^\beta}
   =    C
        \sup_{\substack{x, y \in \Omega \\ x \neq y}}
        \frac{\norm{f(x) - f(y)}}{\norm{x - y}^\beta}
   =    C [f]_{\beta}
\end{align*}
We may replace the constant~$C$ by~$C+1$ to ensure that~$C \geq 1$, while still maintaining that~$[f]_\alpha \leq C [f]_\beta$ for every~$f \colon \Omega \to \Real^m$.
It then further follows that
\[
        \norm{f}_{0,\alpha}
  =     \norm{f}_\infty + [f]_\alpha
  \leq  C \norm{f}_\infty + C [f]_\beta
  =     C \norm{f}_{0,\beta} \,.
\]
It follows in particular for~$f \in \cont^{0,\beta}$ that~$[f]_\alpha \leq C [f]_\beta < \infty$ and hence~$f \in \cont^{0,\alpha}$.





\subsection{}

\begin{lemma}
  \label{subadditive}
  If~$0 \leq \alpha \leq 1$ then the map~$[0,\infty) \to \Real$,~$x \mapsto x^\alpha$  is subadditive, i.e.\ it holds that
  \[
          (x + y)^\alpha
    \leq  x^\alpha + y^\alpha
  \]
  for all~$x, y \in [0,\infty)$.
\end{lemma}

\begin{proof}
  We fix~$x \in [0,\infty)$.
  If~$x = 0$ then the claimed inequality holds, so we may assume that~$x > 0$.
  We then consider the two maps
  \begin{gather*}
            f
    \colon  [0,\infty)
    \to     \Real \,,
    \quad   y
    \mapsto (x + y)^\alpha
  \shortintertext{and}
            g
    \colon  [0,\infty)
    \to     \Real \,,
    \quad   y
    \mapsto x^\alpha + y^\alpha \,.
  \end{gather*}
  It holds that~$f(0) = g(0)$ and and both maps are differentiable.
  It holds for every~$x \in [0,\infty)$ that
  \[
      f'(x)
    =
      \alpha (x+y)^{\alpha-1}
    \leq
      \alpha y^{\alpha - 1}
    =
      g'(x)
  \]
  where we use that~$0 \leq \alpha \leq 1$.
  It therefore follows from~$f(0) = g(0)$ that~$f(x) \leq g(x)$ for all~$x \geq 0$.
\end{proof}

\begin{corollary}
  \label{reverse subadditive}
  It holds for all~$0 \leq \alpha < 1$ and all~$x, y \geq 0$ that
  \[
          \abs{x^\alpha - y^\alpha}
    \leq  \abs{x-y}^\alpha \,.
  \]
\end{corollary}

\begin{proof}
  We may assume that~$x \geq y$.
  Then
  \[
          x^\alpha
    =     ((x - y) + y)^\alpha
    \leq  (x-y)^\alpha + y^\alpha
  \]
  by \cref{subadditive} and therefore
  \[
          \abs{x^\alpha - y^\alpha}
    =     x^\alpha - y^\alpha
    \leq  (x - y)^\alpha
    =     \abs{x-y}^\alpha \,,
  \]
  as desired.
\end{proof}

We first consider the case~$m = 1$.
Fix a base point~$z \in \Omega$ and consider the continuous function
\[
          f
  \colon  \Omega
  \to     \Real \,,
  \quad   x
  \mapsto \norm{x - z}^\alpha \,.
\]
It holds for all~$x, y \in \Omega$ by \cref{reverse subadditive} and the reverse triangle inequality for~$\norm{\,\cdot\,}$ that
\begin{align*}
        \norm{f(x) - f(y)}
  &=    \abs{\, \norm{x-z}^\alpha - \norm{y-z}^\alpha \,} \\
  &\leq \abs{ \, \norm{x-z} - \norm{y-z} \, }^\alpha  \\
  &\leq \abs{ \, \norm{ (x-z) - (y-z) } \, }^\alpha \\
  &\leq \norm{x-y}^\alpha \,.
\end{align*}
It then follows that~$f \in \cont^{0,\alpha}(\Omega)$ because
\[
        [f]_\alpha
  =     \sup_{\substack{x, y \in \Omega \\ x \neq y}}
        \frac{\norm{f(x) - f(y)}}{\norm{x-y}^\alpha}
  \leq  \sup_{\substack{x, y \in \Omega \\ x \neq y}}
        \frac{\norm{x-y}^\alpha}{\norm{x-y}^\alpha}
  =     1 \,.
\]
But~$f \notin \cont^{0,\beta}(\Omega)$ because
\begin{align*}
    [f]_\beta
   =
    \sup_{\substack{x, y \in \Omega \\ x \neq y}}
    \frac{\norm{f(x) - f(y)}}{\norm{x-y}^\beta}
   \mathbin{\underset{y=z}{\geq}}
    \sup_{\substack{x \in \Omega \\ x \neq z}}
    \frac{\norm{f(x) - f(z)}}{\norm{x-z}^\beta}
  &=
    \sup_{\substack{x \in \Omega \\ x \neq z}}
    \frac{\norm{x-z}^\alpha}{\norm{x-z}^\beta}  \\
  &=
    \sup_{\substack{x \in \Omega \\ x \neq z}}
    \frac{1}{\norm{x-z}^{\beta - \alpha}}
   =
    \infty \,,
\end{align*}
where we have used that~$\Omega$ is open and thus contains points arbitrarily close to~$z$ (but distinct to~$z$).

For~$m \geq 1$ we can replace~$f$ by the function
\[
          \Omega
  \to     \Real^m \,,
  \quad   x
  \mapsto \vect{ \norm{x-z}^\alpha \\ 0 \\ \vdots \\ 0 }
\]
and all of the above calculations stay true.





\subsection{}

Every \dash{Hölder}{continuous} function is uniformly continuous, so it sufficies to construct a continuous function~$f \colon \Omega \to \Real^n$ which is not uniformly continuous.
If~$z \in \partial \Omega$ is a boundary point of~$\Omega$ then the function
\[
          f
  \colon  \Omega
  \to     \Real \,,
  \quad   z
  \mapsto \frac{1}{\norm{x-z}}
\]
should do the trick, but I currently don’t have the time to work out the details.



